Checkpoint ExtCall generated driver IH boundary

semantics/prop/vyperTypeStmtSoundnessScript.sml
@@ -9936,23 +9936,9 @@ Proof
   strip_tac >> gvs[]
 QED
 
-Theorem extcall_expr_sound_from_generated_prefix_delayed_ih[local]:
-  !cx env st res st' is_static func_name arg_types ret_type es drv.
-    env_consistent env cx st /\ state_well_typed st /\
-    context_well_typed cx /\ accounts_well_typed st.accounts /\
-    functions_well_typed cx /\
-    well_typed_expr env (Call ret_type (ExtCall is_static (func_name,arg_types,ret_type)) es drv) /\
-    (!env0 st0 res0 st0'.
-       well_typed_exprs env0 es /\ env_consistent env0 cx st0 /\
-       state_well_typed st0 /\ context_well_typed cx /\
-       accounts_well_typed st0.accounts /\ functions_well_typed cx /\
-       eval_exprs cx es st0 = (res0,st0') ==>
-       state_well_typed st0' /\ env_consistent env0 cx st0' /\
-       accounts_well_typed st0'.accounts /\ no_type_error_result res0 /\
-       case res0 of INL vs => exprs_runtime_typed env0 es vs | INR _ => T) /\
-    eval_expr cx (Call ret_type (ExtCall is_static (func_name,arg_types,ret_type)) es drv) st =
-      (res,st') ==>
-    (!s_args vs args_st s_check x_check st_check s_target target_addr st_target
+Definition extcall_generated_driver_ih_def:
+  extcall_generated_driver_ih cx es is_static func_name arg_types drv <=>
+    !s_args vs args_st s_check x_check st_check s_target target_addr st_target
         s_value value_opt arg_vals st_value tenv s_calldata calldata st_calldata
         s_accounts accounts st_accounts s_code x_code st_code s_tstorage tStorage st_tstorage
         txParams caller s_run result st_run success returnData accounts' tStorage'
@@ -9995,14 +9981,72 @@ Theorem extcall_expr_sound_from_generated_prefix_delayed_ih[local]:
            type_place_expr env0 (THE drv) = SOME vt ==>
            state_well_typed st0' /\ env_consistent env0 cx st0' /\
            accounts_well_typed st0'.accounts /\ no_type_error_result res0 /\
-           case res0 of INL tv => place_expr_result_typed env0 tv vt | INR _ => T) ==>
-    state_well_typed st' /\ env_consistent env cx st' /\
-    accounts_well_typed st'.accounts /\ no_type_error_result res /\
-    case res of
-    | INL tv => expr_result_typed env (Call ret_type (ExtCall is_static (func_name,arg_types,ret_type)) es drv) tv
-    | INR _ => T
+           case res0 of INL tv => place_expr_result_typed env0 tv vt | INR _ => T
+End
+
+Theorem extcall_generated_driver_ih_elim_expr[local]:
+  !cx es is_static func_name arg_types drv
+    s_args vs args_st s_check x_check st_check s_target target_addr st_target
+    s_value value_opt arg_vals st_value tenv s_calldata calldata st_calldata
+    s_accounts accounts st_accounts s_code x_code st_code s_tstorage tStorage st_tstorage
+    txParams caller s_run result st_run success returnData accounts' tStorage'
+    s_success x_success st_success s_upd_accounts x_upd_accounts st_upd_accounts
+    s_upd_transient x_upd_transient st_upd_transient.
+    extcall_generated_driver_ih cx es is_static func_name arg_types drv /\
+    eval_exprs cx es s_args = (INL vs,args_st) /\
+    check (vs <> []) "ExtCall no target" s_check = (INL x_check,st_check) /\
+    lift_option_type (dest_AddressV (HD vs)) "ExtCall target not address" s_target =
+      (INL target_addr,st_target) /\
+    (if is_static then return (NONE,TL vs)
+     else do
+       check (TL vs <> []) "ExtCall no value";
+       v <- lift_option_type (dest_NumV (HD (TL vs))) "ExtCall value not int";
+       return (SOME v,TL (TL vs))
+     od) s_value = (INL (value_opt,arg_vals),st_value) /\
+    tenv = get_tenv cx /\
+    lift_option (build_ext_calldata tenv func_name arg_types arg_vals) "ExtCall build_calldata"
+      s_calldata = (INL calldata,st_calldata) /\
+    get_accounts s_accounts = (INL accounts,st_accounts) /\
+    check (~NULL (lookup_account target_addr accounts).code) "ExtCall target has no code" s_code =
+      (INL x_code,st_code) /\
+    get_transient_storage s_tstorage = (INL tStorage,st_tstorage) /\
+    txParams = vyper_to_tx_params cx.txn /\ caller = cx.txn.target /\
+    lift_option (run_ext_call caller target_addr calldata value_opt accounts tStorage txParams)
+      "ExtCall run failed" s_run = (INL result,st_run) /\
+    (success,returnData,accounts',tStorage') = result /\
+    check success "ExtCall reverted" s_success = (INL x_success,st_success) /\
+    update_accounts (K accounts') s_upd_accounts = (INL x_upd_accounts,st_upd_accounts) /\
+    update_transient (K tStorage') s_upd_transient = (INL x_upd_transient,st_upd_transient) ==>
+    (returnData = [] /\ IS_SOME drv ==>
+     !env0 st0 res0 st0'.
+       env_consistent env0 cx st0 /\ state_well_typed st0 /\
+       context_well_typed cx /\ accounts_well_typed st0.accounts /\
+       functions_well_typed cx /\ eval_expr cx (THE drv) st0 = (res0,st0') ==>
+       well_typed_expr env0 (THE drv) ==>
+       state_well_typed st0' /\ env_consistent env0 cx st0' /\
+       accounts_well_typed st0'.accounts /\ no_type_error_result res0 /\
+       case res0 of INL tv => expr_result_typed env0 (THE drv) tv | INR _ => T)
 Proof
-  cheat
+  rpt gen_tac >> strip_tac >>
+  qpat_x_assum `extcall_generated_driver_ih _ _ _ _ _ _` mp_tac >>
+  rewrite_tac[extcall_generated_driver_ih_def] >>
+  disch_then (qspecl_then
+    [`s_args`, `vs`, `args_st`, `s_check`, `x_check`, `st_check`,
+     `s_target`, `target_addr`, `st_target`, `s_value`, `value_opt`,
+     `arg_vals`, `st_value`, `tenv`, `s_calldata`, `calldata`,
+     `st_calldata`, `s_accounts`, `accounts`, `st_accounts`, `s_code`,
+     `x_code`, `st_code`, `s_tstorage`, `tStorage`, `st_tstorage`,
+     `txParams`, `caller`, `s_run`, `result`, `st_run`, `success`,
+     `returnData`, `accounts'`, `tStorage'`, `s_success`, `x_success`,
+     `st_success`, `s_upd_accounts`, `x_upd_accounts`, `st_upd_accounts`,
+     `s_upd_transient`, `x_upd_transient`, `st_upd_transient`]
+    (mk_asm "drv_prefix")) >>
+  strip_tac >> strip_tac >>
+  asm "drv_prefix" mp_tac >>
+  (impl_tac >- metis_tac[]) >> strip_tac >>
+  rpt strip_tac >>
+  first_x_assum (qspecl_then [`env0`, `st0`, `res0`, `st0'`] mp_tac) >>
+  simp[]
 QED
 
 
